spec: split generic reachability from counter case study

packages/zoe/spec/jessie_counter_reach.v
@@ -1,6 +1,6 @@
-(* Reachability lemmas for dynamic authority in the counter case study. *)
+(* Counter-case reachability lemmas over the generic Justin reach relation. *)
 From Coq Require Import Lia List String ZArith.
-Require Import jessie_lang jessie_justin jessie_counter jessie_public.
+Require Import jessie_lang jessie_justin jessie_counter jessie_reach jessie_connectivity.
 
 Import ListNotations.
 Open Scope string_scope.
@@ -10,19 +10,8 @@ Module JessieCounterReach.
   Import Justin.
   Import JustinExec.
   Import JessieCounterCase.
-  Import JessiePublic.
-
-  Inductive reaches_val (σ : state) : val -> val -> Prop :=
-  | ReachesRefl v :
-      reaches_val σ v v
-  | ReachesField l obj fld v w :
-      lookup_obj σ l = Some obj ->
-      lookup_field (obj_fields obj) fld = Some v ->
-      reaches_val σ v w ->
-      reaches_val σ (VLoc l) w.
-
-  Definition reaches_dyn (σ : state) (root : val) (pid : nat) : Prop :=
-    reaches_val σ root (VPrim (PrimDyn pid)).
+  Import JessieReach.
+  Import JessieConnectivity.
 
   Definition dyn_is_entry (σ : state) (pid : nat) : Prop :=
     exists cell, lookup_nat_assoc pid (st_dyn_prims σ) = Some (DynCellDelta cell 1).
@@ -118,207 +107,55 @@ Module JessieCounterReach.
       exists 0%nat. reflexivity.
   Qed.
 
-  Definition builtin_call (p : prim_ref) : Prop :=
-    match p with
-    | PrimBuiltin _ => True
-    | _ => False
-    end.
-
-  Definition result_dyn (e : core_expr) (pid : nat) : Prop :=
-    match e with
-    | CoreVal root => reaches_dyn (State 0%nat 0%nat [] [] [] [] []) root pid
-    | _ => False
-    end.
-
-  Definition conservative_builtin (name : prim_name) : Prop :=
-    forall σ args root σ' pid,
-      apply_prim σ (PrimBuiltin name) args = (CoreVal root, σ') ->
-      reaches_dyn σ' root pid ->
-      exists arg, In arg args /\ reaches_dyn σ arg pid.
-
-  Lemma reaches_val_same_store σ σ' root target :
-    st_store σ = st_store σ' ->
-    reaches_val σ root target ->
-    reaches_val σ' root target.
+  Example makeCounter_result_reaches_fresh_object :
+    val_reaches
+      state_after_makeCounter
+      counter_after_makeCounter
+      (CObj 1%nat).
   Proof.
-    intros Hstore Hreach.
-    induction Hreach as [v|l obj fld v w Hlook Hfield Hsub IH].
+    vm_compute. constructor.
+  Qed.
+
+  Example makeCounter_result_reaches_fresh_incr :
+    val_reaches
+      state_after_makeCounter
+      counter_after_makeCounter
+      (CDyn 0%nat).
+  Proof.
+    vm_compute.
+    econstructor 2.
+    - econstructor 2 with (fld := "incr") (pid := 0%nat).
+      + reflexivity.
+      + reflexivity.
     - constructor.
+  Qed.
+
+  Example makeCounter_result_reaches_fresh_cell :
+    val_reaches
+      state_after_makeCounter
+      counter_after_makeCounter
+      (CCell 0%nat).
+  Proof.
+    vm_compute.
+    econstructor 2.
+    - econstructor 2 with (fld := "incr") (pid := 0%nat).
+      + reflexivity.
+      + reflexivity.
     - econstructor 2.
-      + destruct σ as [next prim store frozen env cells dyn].
-        destruct σ' as [next' prim' store' frozen' env' cells' dyn'].
-        simpl in *. subst store'. exact Hlook.
-      + exact Hfield.
-      + exact IH.
+      + constructor 3.
+        exists 1%nat. reflexivity.
+      + constructor.
   Qed.
 
-  Lemma mark_frozen_preserves_store σ l :
-    st_store (mark_frozen σ l) = st_store σ.
+  Example makeCounter_fresh_refs_satisfy_old_or_fresh :
+    let σ := counter_empty_state in
+    let '(e', σ') := counter_apply_prim σ (PrimExt 0%nat) [] in
+    old_or_fresh σ σ' [] (CObj 1%nat) /\
+    old_or_fresh σ σ' [] (CDyn 0%nat) /\
+    old_or_fresh σ σ' [] (CDyn 1%nat) /\
+    old_or_fresh σ σ' [] (CCell 0%nat).
   Proof.
-    unfold mark_frozen.
-    destruct (existsb (Nat.eqb l) (st_frozen σ)); reflexivity.
-  Qed.
-
-  Lemma freeze_shallow_preserves_store σ v :
-    st_store (freeze_shallow σ v) = st_store σ.
-  Proof.
-    destruct v; simpl; try reflexivity.
-    apply mark_frozen_preserves_store.
-  Qed.
-
-  Lemma freeze_deep_preserves_store fuel σ v :
-    st_store (freeze_deep fuel σ v) = st_store σ.
-  Proof.
-    revert σ v.
-    induction fuel as [|fuel IH]; intros σ v; simpl; [reflexivity|].
-    destruct v; try reflexivity.
-    remember (mark_frozen σ l) as σ1 eqn:Hσ1.
-    assert (Hstore1 : st_store σ1 = st_store σ).
-    { subst σ1. apply mark_frozen_preserves_store. }
-    destruct (lookup_obj σ1 l) as [obj|] eqn:Hobj; [|exact Hstore1].
-    assert (Hfold : forall flds σ0,
-      st_store (fold_left (fun σacc (kv : string * val) => freeze_deep fuel σacc (snd kv)) flds σ0) =
-      st_store σ0).
-    {
-      intros flds.
-      induction flds as [|[k w] rest IHrest]; intros σ0; simpl.
-      - reflexivity.
-      - transitivity (st_store (freeze_deep fuel σ0 w)).
-        + apply IHrest.
-        + apply IH.
-    }
-    rewrite Hfold.
-    exact Hstore1.
-  Qed.
-
-  Lemma reaches_dyn_same_store σ σ' root pid :
-    st_store σ = st_store σ' ->
-    reaches_dyn σ root pid ->
-    reaches_dyn σ' root pid.
-  Proof.
-    unfold reaches_dyn.
-    intros Hstore Hreach.
-    eapply reaches_val_same_store; eauto.
-  Qed.
-
-  Lemma reaches_val_from_lit σ l target :
-    reaches_val σ (VLit l) target ->
-    target = VLit l.
-  Proof.
-    intro Hreach.
-    inversion Hreach; subst; reflexivity.
-  Qed.
-
-  Lemma builtin_assert_conservative :
-    conservative_builtin PrimAssert.
-  Proof.
-    unfold conservative_builtin.
-    intros σ args root σ' pid Happ Hreach.
-    destruct args as [|a args].
-    - cbn in Happ. inversion Happ.
-    - destruct args as [|a2 args].
-      + destruct a as [l|l|p].
-        * destruct l as [j|n|].
-          -- destruct j.
-             ++ cbn in Happ. inversion Happ.
-             ++ destruct b.
-                ** cbn in Happ. inversion Happ; subst; clear Happ.
-                   unfold reaches_dyn in Hreach.
-                   pose proof (reaches_val_from_lit _ _ _ Hreach) as Heq.
-                   discriminate Heq.
-                ** cbn in Happ. inversion Happ.
-             ++ cbn in Happ. inversion Happ.
-             ++ cbn in Happ. inversion Happ.
-             ++ cbn in Happ. inversion Happ.
-             ++ cbn in Happ. inversion Happ.
-          -- cbn in Happ. inversion Happ.
-          -- cbn in Happ. inversion Happ.
-        * cbn in Happ. inversion Happ.
-        * cbn in Happ. inversion Happ.
-      + destruct a as [l|l|p].
-        * destruct l as [j|n|].
-          -- destruct j.
-             ++ cbn in Happ. inversion Happ.
-             ++ destruct b; cbn in Happ; inversion Happ.
-             ++ cbn in Happ. inversion Happ.
-             ++ cbn in Happ. inversion Happ.
-             ++ cbn in Happ. inversion Happ.
-             ++ cbn in Happ. inversion Happ.
-          -- cbn in Happ. inversion Happ.
-          -- cbn in Happ. inversion Happ.
-        * cbn in Happ. inversion Happ.
-        * cbn in Happ. inversion Happ.
-  Qed.
-
-  Lemma builtin_fail_conservative :
-    conservative_builtin PrimFail.
-  Proof.
-    unfold conservative_builtin.
-    intros σ args root σ' pid Happ _.
-    simpl in Happ.
-    discriminate.
-  Qed.
-
-  Lemma builtin_freeze_conservative :
-    conservative_builtin PrimFreeze.
-  Proof.
-    unfold conservative_builtin.
-    intros σ args root σ' pid Happ Hreach.
-    destruct args as [|a args].
-    - cbn in Happ. inversion Happ.
-    - destruct args as [|a2 args].
-      + cbn in Happ. inversion Happ; subst; clear Happ.
-        exists root. split; [left; reflexivity|].
-        eapply (reaches_dyn_same_store (freeze_shallow σ root) σ root pid).
-        * apply freeze_shallow_preserves_store.
-        * exact Hreach.
-      + cbn in Happ. inversion Happ.
-  Qed.
-
-  Lemma builtin_harden_conservative :
-    conservative_builtin PrimHarden.
-  Proof.
-    unfold conservative_builtin.
-    intros σ args root σ' pid Happ Hreach.
-    destruct args as [|a args].
-    - cbn in Happ. inversion Happ.
-    - destruct args as [|a2 args].
-      + cbn in Happ. inversion Happ; subst; clear Happ.
-        exists root. split; [left; reflexivity|].
-        eapply (reaches_dyn_same_store (freeze_deep 20 σ root) σ root pid).
-        * apply freeze_deep_preserves_store.
-        * exact Hreach.
-      + cbn in Happ. inversion Happ.
-  Qed.
-
-  Lemma builtin_id_conservative :
-    conservative_builtin PrimId.
-  Proof.
-    unfold conservative_builtin.
-    intros σ args root σ' pid Happ Hreach.
-    destruct args as [|a args].
-    - cbn in Happ. inversion Happ.
-    - destruct args as [|a2 args].
-      + change ((if hardenedb 20 σ a then (CoreVal a, σ) else (CoreBzzt, σ)) =
-                  (CoreVal root, σ')) in Happ.
-        destruct (hardenedb 20 σ a) eqn:Hhard.
-        * cbn in Happ.
-          inversion Happ; subst; clear Happ.
-          exists root. split; [left; reflexivity|exact Hreach].
-        * cbn in Happ.
-          inversion Happ.
-      + cbn in Happ. inversion Happ.
-  Qed.
-
-  Theorem builtin_conservative (name : prim_name) :
-    conservative_builtin name.
-  Proof.
-    destruct name.
-    - apply builtin_freeze_conservative.
-    - apply builtin_harden_conservative.
-    - apply builtin_assert_conservative.
-    - apply builtin_id_conservative.
-    - apply builtin_fail_conservative.
+    vm_compute. repeat split; now right.
   Qed.
 
   Example entry_cap_root_reaches_only_incr :
@@ -359,30 +196,4 @@ Module JessieCounterReach.
       discriminate.
   Qed.
 
-  Example public_compile_contains_no_dyn (e : JessiePublic.expr) :
-    forall pid,
-      JessiePublic.compile e <> CoreVal (VPrim (PrimDyn pid)).
-  Proof.
-    induction e; intros pid Hc; simpl in Hc; discriminate.
-  Qed.
-
-  Example freeze_is_conservative :
-    conservative_builtin PrimFreeze.
-  Proof. apply builtin_conservative. Qed.
-
-  Example harden_is_conservative :
-    conservative_builtin PrimHarden.
-  Proof. apply builtin_conservative. Qed.
-
-  Example assert_is_conservative :
-    conservative_builtin PrimAssert.
-  Proof. apply builtin_conservative. Qed.
-
-  Example id_is_conservative :
-    conservative_builtin PrimId.
-  Proof. apply builtin_conservative. Qed.
-
-  Example fail_is_conservative :
-    conservative_builtin PrimFail.
-  Proof. apply builtin_conservative. Qed.
 End JessieCounterReach.
