packages/zoe/spec/jessie_reach.v
@@ -1,0 +1,243 @@
+(* Generic reachability lemmas for dynamic authority in the Justin core. *)
+From Coq Require Import Lia List String ZArith.
+Require Import jessie_lang jessie_justin jessie_public.
+
+Import ListNotations.
+Open Scope string_scope.
+Open Scope Z_scope.
+
+Module JessieReach.
+  Import Justin.
+  Import JustinExec.
+  Import JessiePublic.
+
+  Inductive reaches_val (σ : state) : val -> val -> Prop :=
+  | ReachesRefl v :
+      reaches_val σ v v
+  | ReachesField l obj fld v w :
+      lookup_obj σ l = Some obj ->
+      lookup_field (obj_fields obj) fld = Some v ->
+      reaches_val σ v w ->
+      reaches_val σ (VLoc l) w.
+
+  Definition reaches_dyn (σ : state) (root : val) (pid : nat) : Prop :=
+    reaches_val σ root (VPrim (PrimDyn pid)).
+
+  Lemma reaches_val_same_store σ σ' root target :
+    st_store σ = st_store σ' ->
+    reaches_val σ root target ->
+    reaches_val σ' root target.
+  Proof.
+    intros Hstore Hreach.
+    induction Hreach as [v|l obj fld v w Hlook Hfield Hsub IH].
+    - constructor.
+    - econstructor 2.
+      + destruct σ as [next prim store frozen env cells dyn].
+        destruct σ' as [next' prim' store' frozen' env' cells' dyn'].
+        simpl in *. subst store'. exact Hlook.
+      + exact Hfield.
+      + exact IH.
+  Qed.
+
+  Lemma mark_frozen_preserves_store σ l :
+    st_store (mark_frozen σ l) = st_store σ.
+  Proof.
+    unfold mark_frozen.
+    destruct (existsb (Nat.eqb l) (st_frozen σ)); reflexivity.
+  Qed.
+
+  Lemma freeze_shallow_preserves_store σ v :
+    st_store (freeze_shallow σ v) = st_store σ.
+  Proof.
+    destruct v; simpl; try reflexivity.
+    apply mark_frozen_preserves_store.
+  Qed.
+
+  Lemma freeze_deep_preserves_store fuel σ v :
+    st_store (freeze_deep fuel σ v) = st_store σ.
+  Proof.
+    revert σ v.
+    induction fuel as [|fuel IH]; intros σ v; simpl; [reflexivity|].
+    destruct v; try reflexivity.
+    remember (mark_frozen σ l) as σ1 eqn:Hσ1.
+    assert (Hstore1 : st_store σ1 = st_store σ).
+    { subst σ1. apply mark_frozen_preserves_store. }
+    destruct (lookup_obj σ1 l) as [obj|] eqn:Hobj; [|exact Hstore1].
+    assert (Hfold : forall flds σ0,
+      st_store (fold_left (fun σacc (kv : string * val) => freeze_deep fuel σacc (snd kv)) flds σ0) =
+      st_store σ0).
+    {
+      intros flds.
+      induction flds as [|[k w] rest IHrest]; intros σ0; simpl.
+      - reflexivity.
+      - transitivity (st_store (freeze_deep fuel σ0 w)).
+        + apply IHrest.
+        + apply IH.
+    }
+    rewrite Hfold.
+    exact Hstore1.
+  Qed.
+
+  Lemma reaches_dyn_same_store σ σ' root pid :
+    st_store σ = st_store σ' ->
+    reaches_dyn σ root pid ->
+    reaches_dyn σ' root pid.
+  Proof.
+    unfold reaches_dyn.
+    intros Hstore Hreach.
+    eapply reaches_val_same_store; eauto.
+  Qed.
+
+  Lemma reaches_val_from_lit σ l target :
+    reaches_val σ (VLit l) target ->
+    target = VLit l.
+  Proof.
+    intro Hreach.
+    inversion Hreach; subst; reflexivity.
+  Qed.
+
+  Definition conservative_builtin (name : prim_name) : Prop :=
+    forall σ args root σ' pid,
+      apply_prim σ (PrimBuiltin name) args = (CoreVal root, σ') ->
+      reaches_dyn σ' root pid ->
+      exists arg, In arg args /\ reaches_dyn σ arg pid.
+
+  Lemma builtin_assert_conservative :
+    conservative_builtin PrimAssert.
+  Proof.
+    unfold conservative_builtin.
+    intros σ args root σ' pid Happ Hreach.
+    destruct args as [|a args].
+    - cbn in Happ. inversion Happ.
+    - destruct args as [|a2 args].
+      + destruct a as [l|l|p].
+        * destruct l as [j|n|].
+          -- destruct j.
+             ++ cbn in Happ. inversion Happ.
+             ++ destruct b.
+                ** cbn in Happ. inversion Happ; subst; clear Happ.
+                   unfold reaches_dyn in Hreach.
+                   pose proof (reaches_val_from_lit _ _ _ Hreach) as Heq.
+                   discriminate Heq.
+                ** cbn in Happ. inversion Happ.
+             ++ cbn in Happ. inversion Happ.
+             ++ cbn in Happ. inversion Happ.
+             ++ cbn in Happ. inversion Happ.
+             ++ cbn in Happ. inversion Happ.
+          -- cbn in Happ. inversion Happ.
+          -- cbn in Happ. inversion Happ.
+        * cbn in Happ. inversion Happ.
+        * cbn in Happ. inversion Happ.
+      + destruct a as [l|l|p].
+        * destruct l as [j|n|].
+          -- destruct j.
+             ++ cbn in Happ. inversion Happ.
+             ++ destruct b; cbn in Happ; inversion Happ.
+             ++ cbn in Happ. inversion Happ.
+             ++ cbn in Happ. inversion Happ.
+             ++ cbn in Happ. inversion Happ.
+             ++ cbn in Happ. inversion Happ.
+          -- cbn in Happ. inversion Happ.
+          -- cbn in Happ. inversion Happ.
+        * cbn in Happ. inversion Happ.
+        * cbn in Happ. inversion Happ.
+  Qed.
+
+  Lemma builtin_fail_conservative :
+    conservative_builtin PrimFail.
+  Proof.
+    unfold conservative_builtin.
+    intros σ args root σ' pid Happ _.
+    simpl in Happ.
+    discriminate.
+  Qed.
+
+  Lemma builtin_freeze_conservative :
+    conservative_builtin PrimFreeze.
+  Proof.
+    unfold conservative_builtin.
+    intros σ args root σ' pid Happ Hreach.
+    destruct args as [|a args].
+    - cbn in Happ. inversion Happ.
+    - destruct args as [|a2 args].
+      + cbn in Happ. inversion Happ; subst; clear Happ.
+        exists root. split; [left; reflexivity|].
+        eapply (reaches_dyn_same_store (freeze_shallow σ root) σ root pid).
+        * apply freeze_shallow_preserves_store.
+        * exact Hreach.
+      + cbn in Happ. inversion Happ.
+  Qed.
+
+  Lemma builtin_harden_conservative :
+    conservative_builtin PrimHarden.
+  Proof.
+    unfold conservative_builtin.
+    intros σ args root σ' pid Happ Hreach.
+    destruct args as [|a args].
+    - cbn in Happ. inversion Happ.
+    - destruct args as [|a2 args].
+      + cbn in Happ. inversion Happ; subst; clear Happ.
+        exists root. split; [left; reflexivity|].
+        eapply (reaches_dyn_same_store (freeze_deep 20 σ root) σ root pid).
+        * apply freeze_deep_preserves_store.
+        * exact Hreach.
+      + cbn in Happ. inversion Happ.
+  Qed.
+
+  Lemma builtin_id_conservative :
+    conservative_builtin PrimId.
+  Proof.
+    unfold conservative_builtin.
+    intros σ args root σ' pid Happ Hreach.
+    destruct args as [|a args].
+    - cbn in Happ. inversion Happ.
+    - destruct args as [|a2 args].
+      + change ((if hardenedb 20 σ a then (CoreVal a, σ) else (CoreBzzt, σ)) =
+                  (CoreVal root, σ')) in Happ.
+        destruct (hardenedb 20 σ a) eqn:Hhard.
+        * cbn in Happ.
+          inversion Happ; subst; clear Happ.
+          exists root. split; [left; reflexivity|exact Hreach].
+        * cbn in Happ.
+          inversion Happ.
+      + cbn in Happ. inversion Happ.
+  Qed.
+
+  Theorem builtin_conservative (name : prim_name) :
+    conservative_builtin name.
+  Proof.
+    destruct name.
+    - apply builtin_freeze_conservative.
+    - apply builtin_harden_conservative.
+    - apply builtin_assert_conservative.
+    - apply builtin_id_conservative.
+    - apply builtin_fail_conservative.
+  Qed.
+
+  Example public_compile_contains_no_dyn (e : JessiePublic.expr) :
+    forall pid,
+      JessiePublic.compile e <> CoreVal (VPrim (PrimDyn pid)).
+  Proof.
+    induction e; intros pid Hc; simpl in Hc; discriminate.
+  Qed.
+
+  Example freeze_is_conservative :
+    conservative_builtin PrimFreeze.
+  Proof. apply builtin_conservative. Qed.
+
+  Example harden_is_conservative :
+    conservative_builtin PrimHarden.
+  Proof. apply builtin_conservative. Qed.
+
+  Example assert_is_conservative :
+    conservative_builtin PrimAssert.
+  Proof. apply builtin_conservative. Qed.
+
+  Example id_is_conservative :
+    conservative_builtin PrimId.
+  Proof. apply builtin_conservative. Qed.
+
+  Example fail_is_conservative :
+    conservative_builtin PrimFail.
+  Proof. apply builtin_conservative. Qed.
+End JessieReach.
